refinement from SAT_l to SAT_wl

Weidenbach_Book/Watched_Literals_Watch_List_Domain_Restart.thy
@@ -1098,12 +1098,17 @@ lemma cdcl_twl_stgy_restart_prog_wl_D_cdcl_twl_stgy_restart_prog_wl:
   done
 
 
+definition cdcl_twl_stgy_restart_abs_wl_D_inv where
+  \<open>cdcl_twl_stgy_restart_abs_wl_D_inv S0 brk T n \<longleftrightarrow>
+    cdcl_twl_stgy_restart_abs_wl_inv S0 brk T n \<and>
+    literals_are_\<L>\<^sub>i\<^sub>n (all_atms_st T) T\<close>
+  
 definition cdcl_twl_stgy_restart_prog_early_wl_D
   :: "nat twl_st_wl \<Rightarrow> nat twl_st_wl nres"
 where
   \<open>cdcl_twl_stgy_restart_prog_early_wl_D S\<^sub>0 = do {
     ebrk \<leftarrow> RES UNIV;
-    (ebrk, brk, T, n) \<leftarrow> WHILE\<^sub>T\<^bsup>\<lambda>(_, brk, T, n). cdcl_twl_stgy_restart_abs_wl_inv S\<^sub>0 brk T n\<^esup>
+    (ebrk, brk, T, n) \<leftarrow> WHILE\<^sub>T\<^bsup>\<lambda>(_, brk, T, n). cdcl_twl_stgy_restart_abs_wl_D_inv S\<^sub>0 brk T n\<^esup>
       (\<lambda>(ebrk, brk, _). \<not>brk \<and> \<not>ebrk)
       (\<lambda>(_, brk, S, n).
       do {
@@ -1115,7 +1120,7 @@ where
       })
       (ebrk, False, S\<^sub>0::nat twl_st_wl, 0);
     if \<not>brk then do {
-      (brk, T, _) \<leftarrow> WHILE\<^sub>T\<^bsup>\<lambda>(brk, T, n). cdcl_twl_stgy_restart_abs_wl_inv S\<^sub>0 brk T n\<^esup>
+      (brk, T, _) \<leftarrow> WHILE\<^sub>T\<^bsup>\<lambda>(brk, T, n). cdcl_twl_stgy_restart_abs_wl_D_inv S\<^sub>0 brk T n\<^esup>
 	(\<lambda>(brk, _). \<not>brk)
 	(\<lambda>(brk, S, n).
 	do {
@@ -1147,6 +1152,7 @@ lemma cdcl_twl_stgy_restart_prog_early_wl_D_cdcl_twl_stgy_restart_prog_early_wl:
       WHILEIT_refine[where R=\<open>bool_rel \<times>\<^sub>r {(S, T). (S, T) \<in> Id \<and>
         literals_are_\<L>\<^sub>i\<^sub>n (all_atms_st S) S} \<times>\<^sub>r nat_rel\<close>])
   subgoal by auto
+  subgoal unfolding  cdcl_twl_stgy_restart_abs_wl_D_inv_def by auto
   subgoal by auto
   subgoal by auto
   subgoal by auto
@@ -1154,8 +1160,7 @@ lemma cdcl_twl_stgy_restart_prog_early_wl_D_cdcl_twl_stgy_restart_prog_early_wl:
   subgoal by auto
   subgoal by auto
   subgoal by auto
-  subgoal by auto
-  subgoal by auto
+  subgoal unfolding  cdcl_twl_stgy_restart_abs_wl_D_inv_def by auto
   subgoal by auto
   subgoal by auto
   subgoal by auto
